Compile.v
@@ -1,94 +1,257 @@
 (** This is the top level driver for the compiler. *)
 
 From Coq Require Import String List ListSet Arith NArith.
-From Vyper Require Import Config Calldag.
+From Vyper Require Import Config Calldag ProtoAST.
 From Vyper.L10 Require AST Callset Descend Interpret.
 From Vyper.From10To20 Require FunCtx Call.
 From Vyper.From20To30 Require FunCtx Call.
+From Vyper.From30To40 Require Translate FunCtx Call.
+From Vyper.From40To50 Require Translate Call.
+From Vyper.From40To50 Require Import Proto.
+From Vyper.L40Metered Require Call.
 From Vyper.CheckArith Require Builtins Translate Call.
 From Vyper Require Import ConstFold L10.Base.
+From Vyper.L50 Require Import Types.
 
-(** This is the verified part of the compiler.
-    This function translates a L10 calldag into a L30 calldag (or an error).
+(** This is the part of the compiler that uses calldags,
+      which are declaration maps annotated with maximum possible call depth.
+    It starts with L10 (a subset of Fe/Vyper) and reaches L40 (a precursor to Yul).
+    This part is defined separately here because the theorem verifying it (the next one)
+    looks nice and clean compared to what happens at the final step from L40 to L50.
  *)
-Definition translate_10_to_30 {C: VyperConfig} (B: CheckArith.Builtins.builtin_names_config)
+Definition translate_10_to_40 {C: VyperConfig}
+                              (B: CheckArith.Builtins.builtin_names_config)
                               (calldag10: L10.Descend.calldag)
-: string + L30.Descend.calldag
-:= let calldag20 := From10To20.FunCtx.translate_calldag calldag10 (* no errors possible *) in
-   match const_fold_calldag calldag20 with
+: string + L40.Descend.calldag
+:= match const_fold_calldag                                                     (* 2nd pass *)
+           (From10To20.FunCtx.translate_calldag calldag10)                      (* 1st pass *)
+   with
    | inl err => inl err
    | inr calldag20' =>
-      match From20To30.FunCtx.translate_calldag calldag20' with
+      match From20To30.FunCtx.translate_calldag calldag20' with                 (* 3rd pass *)
       | inl err => inl err
-      | inr calldag30 => inr (CheckArith.Translate.translate_calldag B calldag30)
+      | inr calldag30 =>
+             From30To40.FunCtx.translate_calldag B                              (* 5th pass *)
+               (CheckArith.Translate.translate_calldag B calldag30)             (* 4th pass *)
       end
    end.
 
-(** This is the theorem verifying that the compiler works as intended.
+(**
+  This theorem verifies the compiler up to L40.
+  The storage is not modeled so [SloadOk] and [SstoreOk] just assert that using storage variables
+  just happens to be the same thing as calling [sload()] and [sstore()].
  *)
-Theorem translate_10_to_30_ok {C: VyperConfig}
+Theorem translate_10_to_40_ok {C: VyperConfig}
                               (B: CheckArith.Builtins.builtin_names_config)
                               (calldag10: L10.Descend.calldag)
-                              (calldag30: L30.Descend.calldag)
-                              (ok: translate_10_to_30 B calldag10 = inr calldag30)
+                              (calldag40: L40.Descend.calldag)
+                              (Ok: translate_10_to_40 B calldag10 = inr calldag40)
                               (builtins: string -> option builtin)
+                              (SloadOk: From30To40.Translate.BuiltinsSupportSload B builtins)
+                              (SstoreOk: From30To40.Translate.BuiltinsSupportSstore B builtins)
                               (BuiltinsOk: Builtins.BuiltinsSupportUInt256 B builtins)
                               (fun_name: string)
                               (world: world_state)
                               (arg_values: list uint256):
-  L30.Interpret.interpret builtins calldag30 fun_name world arg_values
+  L40.Interpret.interpret builtins calldag40 fun_name world arg_values
    =
   L10.Interpret.interpret builtins calldag10 fun_name world arg_values.
 Proof.
+unfold translate_10_to_40 in Ok.
 (* 10 -> 20 *)
 rewrite<- From10To20.Call.translate_ok.
-unfold translate_10_to_30 in ok.
 remember (From10To20.FunCtx.translate_calldag calldag10) as calldag20.
 clear Heqcalldag20.
 
 (* const fold *)
-remember (const_fold_calldag calldag20) as calldag20'. symmetry in Heqcalldag20'.
+remember (const_fold_calldag calldag20) as calldag20'.
+symmetry in Heqcalldag20'.
 destruct calldag20' as [|calldag20']. { discriminate. }
 rewrite<- (const_fold_ok _ Heqcalldag20').
 clear Heqcalldag20'.
 
 (* 20 -> 30 *)
-remember (FunCtx.translate_calldag calldag20') as calldag30_ops. symmetry in Heqcalldag30_ops.
-destruct calldag30_ops as [|calldag30_ops]. { discriminate. }
-rewrite<- (From20To30.Call.translate_ok builtins _ _ Heqcalldag30_ops).
-clear Heqcalldag30_ops.
+remember (From20To30.FunCtx.translate_calldag calldag20') as calldag30_pre_arith.
+symmetry in Heqcalldag30_pre_arith.
+destruct calldag30_pre_arith as [|calldag30_pre_arith]. { discriminate. }
+rewrite<- (From20To30.Call.translate_ok builtins _ _ Heqcalldag30_pre_arith).
+clear Heqcalldag30_pre_arith.
 
 (* check arith *)
-inversion ok. subst calldag30.
-apply (CheckArith.Call.translate_ok builtins BuiltinsOk).
+rewrite<- (CheckArith.Call.translate_ok builtins BuiltinsOk).
+remember (CheckArith.Translate.translate_calldag B calldag30_pre_arith) as calldag30.
+clear Heqcalldag30.
+
+(* 30 -> 40 *)
+apply (From30To40.Call.translate_ok builtins _ _ SloadOk SstoreOk BuiltinsOk Ok).
 Qed.
 
-(** This function takes the parser output, which is a list of L10 declarations,
-    and compiles it into a L30 calldag.
 
-    Here [make_calldag] converts the output of the parser to the input to the verified compiler.
+(** This is the verified part of the compiler.
+    It translates a L10 (Fe subset) calldag to L50 (Yul subset).
+    The whole compiler consists of parsing, building a calldag,
+    translating (that's this part) and printing.
+    Since Fe as defined here only has any meaning after the calldag has been built,
+    the verified part must start with the calldag. 
  *)
-Definition compile_to_L30 {C: VyperConfig}
-                          (B: CheckArith.Builtins.builtin_names_config)
-                          (parsed_src: list L10.AST.decl)
-: string + L30.Descend.calldag
-:= match make_calldag L10.AST.decl_name L10.Callset.decl_callset parsed_src with
+Definition translate {C: VyperConfig}
+                     (B: CheckArith.Builtins.builtin_names_config)
+                     (protos: string_map proto)
+                     (calldag10: L10.Descend.calldag)
+: string + string_map L50.AST.fun_decl
+:= match translate_10_to_40 B calldag10 with
    | inl err => inl err
-   | inr cd => translate_10_to_30 B cd
+   | inr calldag40 =>
+        From40To50.Translate.translate_fun_decls B protos (cd_decls calldag40)  (* 6th pass *)
    end.
 
-Definition calldag_to_string {C: VyperConfig} (cd: L30.Descend.calldag)
-:= let _ := string_map_impl in
-   (List.fold_right (fun x tail => x ++ L10.ToString.newline ++ tail) ""
-                    (List.map (fun kv => (L30.AST.string_of_decl (snd kv))) 
-                              (Map.items (cd_decls cd))))%string.
 
-(** This is the compiler without parser. *)
+(** The Yul interpreter needs a maximum call depth,
+    which if exceeded will result in a runtime exception.
+    This function finds a necessary lower bound for this parameter
+    such that this exception can never occur.
+    In principle this value could be extracted from the L10 calldag
+    and proven to not change throughout translate_10_to_40.
+    But this is too complicated and we only care that such a value exists.
+    Therefore, this function simply translates till L40 and gets the value from there.
+ *)
+Definition max_call_depth_lower_bound {C: VyperConfig}
+                                      (B: CheckArith.Builtins.builtin_names_config)
+                                      (calldag10: L10.Descend.calldag)
+: nat
+:= match translate_10_to_40 B calldag10 with
+   | inl err => 0
+   | inr calldag40 => L40Metered.Call.max_depth_in_calldag calldag40
+   end.
+
+(** The Yul interpreter needs a maximum loop iteration count,
+    which if exceeded will result in a runtime exception.
+    Everything in the comment above for [max_call_depth_lower_bound] applies here as well.
+ *)
+Definition max_loop_iters_lower_bound {C: VyperConfig}
+                                      (B: CheckArith.Builtins.builtin_names_config)
+                                      (calldag10: L10.Descend.calldag)
+: N
+:= match translate_10_to_40 B calldag10 with
+   | inl err => 0
+   | inr calldag40 => L40.AST.max_loop_count_decl_map (cd_decls calldag40)
+   end.
+
+(** This is it. This is the proof that the whole thing works.
+    There are a lot of new things happening here compared to [translate_10_to_40_ok] above.
+    There are two sets of builtins now - since Fe and Yul are typed differently - and they must agree.
+    And the compiler needs to know the builtin prototypes so those must agree as well.
+    And the compiler expects some builtins to be there and those expectations must be satisfied too.
+
+    The Yul interpreter needs limits on call depth and loop iterations to be a total function.
+    Those need to be big enough.
+
+    Memory contents might not agree because the Fe interpreter can return results and throw exceptions
+    without modifying memory while the Yul interpreter has to resort to [mstore()] for that.
+    But everything else as provided by the [get_world_except_memory] projection will agree.
+ *)
+Theorem translate_ok {C: VyperConfig}
+                     (B: CheckArith.Builtins.builtin_names_config)
+                     (builtins10: string -> option L10.Base.builtin)
+                     (builtins50: string -> option L50.Builtins.yul_builtin)
+                     (BuiltinsAgree: AllBuiltinsAgreeIfU256 builtins10 builtins50)
+                     (BuiltinsBasics: From40To50.Stmt.BuiltinsSupportBasics builtins50)
+                     (SloadOk: From30To40.Translate.BuiltinsSupportSload B builtins10)
+                     (SstoreOk: From30To40.Translate.BuiltinsSupportSstore B builtins10)
+                     (BuiltinsSafe: forall x,     (* no builtin name may start with '$' *)
+                                      builtins50 ("$" ++ x)%string = None)
+                     (BuiltinsHaveArith: Builtins.BuiltinsSupportUInt256 B builtins10)
+                     {protos: string_map proto}
+                     (KnownProtosOk: check_known_protos B (map_lookup protos) = true)
+                     (ProtosOk: ProtosAgree (map_lookup protos) builtins50)
+
+                     (calldag10: L10.Descend.calldag)
+                     {decls50: string_map L50.AST.fun_decl}
+                     (Ok: translate B protos calldag10 = inr decls50)
+
+                     (max_call_depth: nat)
+                     (max_loop_iters: nat)
+                     (DepthOk:  max_call_depth_lower_bound B calldag10 < max_call_depth)
+                     (ItersOk: (max_loop_iters_lower_bound B calldag10 < N.of_nat max_loop_iters)%N)
+
+                     (fun_name: string)
+                     (world: world_state)
+                     (args: list uint256):
+   let '(world10, result10) := L10.Interpret.interpret builtins10 calldag10 fun_name world args in
+   let '(world50, result50) :=
+      (L50.Call.interpret
+         max_call_depth max_loop_iters
+         builtins50 (map_lookup decls50)
+         ("$" ++ fun_name) world     (* functions are prefixed with '$' to avoid clashes with builtins *)
+         (List.map dynamic_value_of_uint256 args))       (* args are converted into Yul dynamic values *)
+   in
+     get_world_except_memory world10 = get_world_except_memory world50
+      /\
+     match result10 with (* Yul returns a list of dynamic values so just result10 = result50 won't do *)
+     | ExprAbort a    =>  result50 = Some (ExprAbort a)  (* 'Some' means that we're not out of limits *)
+     | ExprSuccess v  =>  result50 = Some (ExprSuccess (dynamic_value_of_uint256 v :: nil))
+     end.
+Proof.
+unfold translate in Ok.
+remember (translate_10_to_40 B calldag10) as calldag40. symmetry in Heqcalldag40.
+destruct calldag40 as [|calldag40]. { discriminate. }
+rewrite<- (translate_10_to_40_ok B calldag10 calldag40 Heqcalldag40 builtins10
+           SloadOk SstoreOk BuiltinsHaveArith fun_name world args).
+unfold max_call_depth_lower_bound in DepthOk. rewrite Heqcalldag40 in DepthOk.
+unfold max_loop_iters_lower_bound in ItersOk. rewrite Heqcalldag40 in ItersOk.
+assert (M := L40Metered.Call.metering_ok DepthOk builtins10 fun_name world args).
+destruct (Interpret.interpret builtins10 calldag40 fun_name world args) as (world10, result10).
+assert (T := From40To50.Call.translate_ok max_call_depth max_loop_iters builtins10 builtins50
+                                          BuiltinsAgree BuiltinsBasics BuiltinsSafe BuiltinsHaveArith
+                                          KnownProtosOk ProtosOk Ok ItersOk
+                                          fun_name world args).
+rewrite M in T. clear M.
+unfold dynamic_value_of_uint256.
+destruct L50.Call.interpret as (world50, result50).
+unfold From40To50.Expr.ResultsAgree in T.
+destruct result50 as [result50|]. 2:easy.
+destruct T as (T, E).
+unfold ExprResultsAgree in E.
+destruct result10 as [v10|a10], result50 as [v50|a50]; try easy.
+2:{ (* double abort *) subst a50. destruct a10; now subst. }
+(* double success *)
+destruct v50. 1:easy.
+destruct v50. 2:easy.
+destruct E as (E, _).
+now subst.
+Qed.
+
+(** This function takes the parser output, which is a list of L10 declarations, and compiles it to L50.
+
+    Here [make_calldag] converts the output of the parser to the input to the verified compiler,
+    checking for duplicated names and call cycles.
+ *)
+Definition compile_to_L50 {C: VyperConfig}
+                          (B: CheckArith.Builtins.builtin_names_config)
+                          (protos: string_map proto)
+                          (parsed_src: list L10.AST.decl)
+: string + string_map L50.AST.fun_decl
+:= match make_calldag L10.AST.decl_name L10.Callset.decl_callset parsed_src with
+   | inl err => inl err
+   | inr cd => translate B protos cd
+   end.
+
+Definition string_of_fun_decls {C: VyperConfig} (d: string_map L50.AST.fun_decl)
+:= (let newline := "
+" in List.fold_right (fun x tail => x ++ newline ++ tail) "" (L50.AST.lines_of_fun_decls d))%string.
+
+(** This is the compiler without parsers (for the prototypes and for Fe).
+    Both parsers are implemented with the usual Haskell tools, alex and happy.
+ *)
 Definition compile {C: VyperConfig}
                    (B: CheckArith.Builtins.builtin_names_config)
+                   (parsed_proto: list proto_ast)
                    (parsed_src: list L10.AST.decl)
 : string + string
-:= match compile_to_L30 B parsed_src with
+:= match make_proto_table parsed_proto with
    | inl err => inl err
-   | inr cd => inr (calldag_to_string cd)
+   | inr protos => match compile_to_L50 B protos parsed_src with
+                   | inl err => inl err
+                   | inr d => inr (string_of_fun_decls d)
+                   end
    end.
