From30To40/Call.v
@@ -122,6 +122,140 @@ now rewrite (let _ := memory_impl in
                                        nil).
 Qed.
 
-(* I won't deal with make_fun_ctx_and_bound_ok here
-   because the next step is to change the evaluation metering.
- *)
+Lemma match_some {T R} {x: option T} {y: T} (E: x = Some y)
+                 (some_branch: forall z: T, x = Some z -> R)
+                 (none_branch: x = None -> R):
+  match x as x' return x = x' -> _ with
+  | Some z => some_branch z
+  | None => none_branch
+  end eq_refl
+   =
+  some_branch y E.
+Proof.
+destruct x. 2:discriminate.
+inversion E. subst. f_equal. apply proof_irrelevance.
+Qed.
+
+Lemma match_none {T R} {x: option T} (E: x = None)
+                 (some_branch: forall z: T, x = Some z -> R)
+                 (none_branch: x = None -> R):
+  match x as x' return x = x' -> _ with
+  | Some z => some_branch z
+  | None => none_branch
+  end eq_refl
+   =
+  none_branch E.
+Proof.
+destruct x. 1:discriminate.
+inversion E. subst. f_equal. apply proof_irrelevance.
+Qed.
+
+
+Local Lemma is_fun_to_not_var_decl {C: VyperConfig}
+                                   (cd30: L30.Descend.calldag)
+                                   (fun_name: string)
+                                   (IsFun: match cd_declmap cd30 fun_name with
+                                           | Some (L30.AST.FunDecl _ _ _) => True
+                                           | _ => False
+                                           end)
+                                   (b: {bound : nat & fun_ctx cd30 bound})
+                                   (FC: make_fun_ctx_and_bound cd30 fun_name = Some b):
+  forall x,
+    fun_decl (projT2 b) <> AST.StorageVarDecl x.
+Proof.
+unfold make_fun_ctx_and_bound in FC.
+refine (match cd_declmap cd30 fun_name as z return _ = z -> _ with
+        | Some (L30.AST.FunDecl name arity body) => fun E => _
+        | _ => fun E => _
+        end eq_refl); rewrite E in IsFun; try contradiction.
+rewrite (match_some E) in FC.
+refine (match cd_depthmap cd30 fun_name as z return _ = z -> _ with
+        | Some depth => fun Edepth => _
+        | _ => fun Edepth => _
+        end eq_refl).
+2:{ rewrite (match_none Edepth) in FC. exfalso. apply (Calldag.make_fun_ctx_helper E Edepth). }
+rewrite (match_some Edepth) in FC.
+inversion FC. subst b. clear FC.
+cbn.
+intros x H. discriminate.
+Qed.
+
+Theorem translate_ok {C: VyperConfig}
+                     {B: builtin_names_config}
+                     (builtins: string -> option builtin)
+                     (cd30: L30.Descend.calldag)
+                     (cd40: L40.Descend.calldag)
+                     (SloadOk: BuiltinsSupportSload B builtins)
+                     (SstoreOk: BuiltinsSupportSstore B builtins)
+                     (BuiltinsOk: BuiltinsSupportUInt256 B builtins)
+                     (Ok: translate_calldag B cd30 = inr cd40)
+                     (fun_name: string)
+                     (world: world_state)
+                     (arg_values: list uint256):
+  L40.Interpret.interpret builtins cd40 fun_name world arg_values
+   =
+  L30.Interpret.interpret builtins cd30 fun_name world arg_values.
+Proof.
+assert (T := translate_fun_ctx_declmap B Ok fun_name).
+unfold L30.Interpret.interpret. unfold L40.Interpret.interpret.
+unfold make_fun_ctx_and_bound.
+refine (match cd_declmap cd30 fun_name as z return _ = z -> _ with
+        | Some (L30.AST.FunDecl name30 arity30 body30) => fun E30 => _
+        | _ => fun E30 => _
+        end eq_refl); rewrite E30 in T;
+  refine (match cd_declmap cd40 fun_name as z return _ = z -> _ with
+          | Some (L40.AST.FunDecl name40 arity40 (AST.Block body40)) => fun E40 => _
+          | None => fun E40 => _
+          end eq_refl); rewrite E40 in T; try discriminate.
+{ (* var decl *)
+  rewrite (match_some E30). rewrite (match_none E40).
+  refine (match cd_depthmap cd30 fun_name as z return _ = z -> _ with
+          | Some depth => fun Edepth => _
+          | _ => fun Edepth => _
+          end eq_refl).
+  2:{ exfalso. apply (Calldag.make_fun_ctx_helper E30 Edepth). }
+  now rewrite (match_some Edepth).
+}
+2:{ (* nothing *) rewrite (match_none E30). rewrite (match_none E40). trivial. }
+(* function *)
+rewrite (match_some E30). rewrite (match_some E40).
+refine (match cd_depthmap cd30 fun_name as z return _ = z -> _ with
+        | Some depth => fun Edepth => _
+        | _ => fun Edepth => _
+        end eq_refl).
+2:{ exfalso. apply (Calldag.make_fun_ctx_helper E30 Edepth). }
+rewrite (match_some Edepth).
+assert (D := translate_fun_ctx_depthmap B Ok fun_name).
+rewrite Edepth in D.
+rewrite (match_some D).
+assert (OkBody: translate_stmt B (cd_decls cd30) body30 = inr body40) by now inversion T.
+remember ({|
+    fun_name := fun_name;
+    fun_depth := depth;
+    fun_depth_ok := Edepth;
+    fun_decl := L30.AST.FunDecl name30 arity30 body30;
+    fun_decl_ok := E30;
+    fun_bound_ok := proj2 (Nat.ltb_lt depth (S depth)) (Nat.lt_succ_diag_r depth)
+  |}) as fc30.
+remember ({|
+    fun_name := fun_name;
+    fun_depth := depth;
+    fun_depth_ok := D;
+    fun_decl := AST.FunDecl name40 arity40 (AST.Block body40);
+    fun_decl_ok := E40;
+    fun_bound_ok := proj2 (Nat.ltb_lt depth (S depth)) (Nat.lt_succ_diag_r depth)
+  |}) as fc40.
+assert (FcNotVar: forall x : string, fun_decl fc30 <> AST.StorageVarDecl x).
+{ subst. intros x H. cbn in H. discriminate. }
+assert (P := FunCtx.translate_fun_ctx_decl_ok fc30 B Ok FcNotVar).
+replace (Calldag.fun_name fc30) with fun_name in P by now subst.
+assert (F: fc40 = translate_fun_ctx fc30 B Ok FcNotVar).
+{
+  subst. unfold translate_fun_ctx. cbn.
+  rewrite E40 in P.
+  remember (AST.FunDecl name40 arity40 (AST.Block body40)) as f. clear Heqf. 
+  inversion P; subst f.
+  f_equal; apply proof_irrelevance.
+}
+rewrite F. now apply interpret_translated_call.
+Qed.
