L50/AST.v
@@ -1,4 +1,4 @@
-From Coq Require Import String.
+From Coq Require Import String HexString ZArith.
 From Vyper Require Import Config.
 From Vyper.L50 Require Import Types.
 
@@ -49,3 +49,125 @@ Next Obligation.
 destruct s; cbn in IsVarDecl; try discriminate.
 exact (H vars init eq_refl).
 Qed.
+
+(****************************   print   ******************************)
+
+Local Open Scope list_scope.
+Local Open Scope string_scope.
+
+Fixpoint to_comma_list {A} (s: A -> string) (l: list A)
+: string
+:= match l with
+   | nil => ""
+   | x :: nil => s x
+   | h :: t => s h ++ ", " ++ to_comma_list s t
+   end.
+
+Definition string_of_typename (tn: typename)
+:= let '(t, n) := tn in
+   n ++ ":" ++ string_of_type t.
+
+Definition string_of_yul_value {C: VyperConfig} {t: yul_type} (v: yul_value t)
+:= match v with
+   | NumberValue _ value _ => HexString.of_Z (Z_of_uint256 value)
+   | BoolValue _ true _ => "true"
+   | BoolValue _ false _ => "false"
+   end.
+
+Fixpoint string_of_expr {C: VyperConfig} (e: expr)
+:= match e with
+   | FunCall name args => (name ++ "(" ++
+                          (* Coq won't allow to_comma_list here *)
+                          (fix string_of_exprs (l: list expr) :=
+                             match l with
+                             | nil => ""
+                             | x :: nil => string_of_expr x
+                             | h :: t => string_of_expr h ++ ", " ++ string_of_exprs t
+                             end) args
+                            ++ ")")%string
+   | LocVar name => name
+   | Const t v => string_of_yul_value v ++ ":" ++ string_of_type t
+   end.
+
+Definition attach (a b: list string)
+: list string
+:= match b with
+   | nil => a
+   | hb :: tb =>
+     let a' := List.rev a in
+       match a' with
+       | nil => b
+       | ha :: ta => List.rev ta ++ (ha ++ " " ++ hb) :: tb
+       end
+   end.
+
+Fixpoint lines_of_stmt {C: VyperConfig} (s: stmt)
+: list string
+:= match s with
+   | BlockStmt b => lines_of_block b
+   | VarDecl vars init => ("let " ++ to_comma_list string_of_typename vars
+                             ++ match init with
+                                | Some e => " := " ++ string_of_expr e
+                                | None => ""
+                                end) :: nil
+   | Assign lhs rhs => (to_comma_list id lhs ++ " := " ++ string_of_expr rhs) :: nil
+   | If cond body => ("if " ++ string_of_expr cond) :: lines_of_block body
+   | Expr e => string_of_expr e :: nil
+   | Switch e cases default =>
+      ("switch " ++ string_of_expr e) ::
+      (fix lines_of_cases (l: list case): list string :=
+        match l with
+        | nil => nil
+        | h :: t => (lines_of_case h ++ lines_of_cases t)%list
+        end) cases ++
+       match default with
+       | None => nil
+       | Some def => "default" :: lines_of_block def
+       end
+   | For init cond inc body => attach ("for" :: nil)
+                                      (attach (lines_of_block init)
+                                              (attach (string_of_expr cond :: nil)
+                                                      (lines_of_block inc)))
+                                ++ lines_of_block body
+   | Break => "break" :: nil
+   | Continue => "continue" :: nil
+   | Leave => "leave" :: nil
+   end
+with lines_of_case {C: VyperConfig} (c: case)
+: list string
+:= let '(Case t v body) := c in
+   ("case " ++ string_of_yul_value v ++ ":" ++ string_of_type t) :: lines_of_block body
+with lines_of_block {C: VyperConfig} (b: block)
+: list string
+:= let fix lines_of_stmts (l: list stmt) :=
+          match l with
+          | nil => nil
+          | h :: t => (lines_of_stmt h ++ lines_of_stmts t)%list
+          end in
+   let '(Block stmts) := b in
+   let lines := lines_of_stmts stmts in
+   match lines with
+   | nil => "{}" :: nil
+   | line :: nil => ("{ " ++ line ++ " }") :: nil
+   | _ => "{" :: List.map (fun x => "    " ++ x) lines ++ "}" :: nil
+   end.
+
+(** Name override is needed because fd_name not properly mangled.
+    (Actually fun_decl has no reason to store its name at all.)
+ *)
+Definition lines_of_fun_decl {C: VyperConfig} (fd: fun_decl) (override_name: string)
+:= ("function " ++ override_name ++ 
+      "(" ++ to_comma_list string_of_typename (fd_inputs fd) ++ ")" ++
+      match fd_outputs fd with
+      | nil => ""
+      | _ => " -> " ++ to_comma_list string_of_typename (fd_outputs fd)
+      end)
+   :: lines_of_block (fd_body fd).
+
+Definition lines_of_fun_decls {C: VyperConfig} (decls: string_map fun_decl)
+:= let _ := string_map_impl in
+   (fix lines_of_alist (l: list (string * fun_decl))
+    := match l with
+       | nil => nil
+       | h :: t => let '(k, v) := h in (lines_of_fun_decl v k ++ lines_of_alist t)%list
+       end) (Map.items decls).
